new/proof/go_etcd_io/raft/v3.v
@@ -5,6 +5,28 @@ From New.proof.go_etcd_io.raft.v3_proof Require Export base protocol.
 From New.proof Require Import grove_prelude.
 
 Section proof.
-Context `{!heapGS Σ}.
+Context `{hG: heapGS Σ, !ffi_semantics _ _}.
+Context `{!globalsGS Σ} {go_ctx : GoContext}.
+Context `{!contextG Σ}.
+
+Definition is_Node (γ : raft_names) (n : raft.Node.t) : iProp Σ :=
+  ∃ (n_ptr : loc),
+    "%Hn" ∷ ⌜ n = interface.mk (ptrT.id raft.node.id) #n_ptr ⌝ ∗
+    "#Hnode" ∷ is_node γ n_ptr.
+
+Lemma wp_Node__Propose  ctx ctx_desc n γraft data_sl data :
+  {{{ is_pkg_init raft ∗
+      "#Hctx" ∷ is_Context ctx ctx_desc ∗
+      "#Hnode" ∷ is_Node γraft n ∗
+      "data_sl" ∷ data_sl ↦* data ∗
+      "Hupd" ∷ (|={⊤,∅}=> ∃ log, own_raft_log γraft log ∗ (own_raft_log γraft (log ++ [data]) ={∅,⊤}=∗ True))
+  }}}
+    interface.get #"Propose" #n #ctx #data_sl
+  {{{ (err : error.t), RET #err; True }}}.
+Proof.
+  wp_start. iNamed "Hpre". iNamed "Hnode". subst.
+  wp_auto. wp_apply (wp_node__Propose with "[$]").
+  iIntros (?) "_". by iApply "HΦ".
+Qed.
 
 End proof.
